Tutorial/Grind/IndexMap.lean
@@ -31,10 +31,10 @@ set_option verso.exampleProject "."
 set_option verso.exampleModule "IndexMapGrind"
 
 
-#doc (Tutorial) "`IndexMap`" =>
+#doc (Tutorial) "Using `grind` for Ordered Maps" =>
 %%%
 slug := "grind-index-map"
-summary := "A walkthrough of ..."
+summary := "A demonstration of how to use `grind` to automate essentially all proofs in a new data structure, with an interface that finds proofs automatically."
 exampleStyle := .inlineLean `IndexMap
 %%%
 
